

Core Equations — asdf

Jerich Lee

2025-11-04

$$144p_xV_x = RT_x \quad (1.9)$$

$$\frac{1}{2gJ}(v_x^2 - v_i^2) = C_p(T_i - T_x) \quad (1.10)$$

$$\frac{A_iv_i}{144V_i} = \frac{A_xv_x}{144V_x} \quad (1.11)$$

$$p_iV_i^\gamma = p_xV_x^\gamma \quad (1.12)$$

$$\frac{(p_{inj})}{(p_{cns})} = \frac{(1 + \gamma M_i^2)}{(1 + \frac{\gamma-1}{2} M_i^2)^{\frac{\gamma}{\gamma-1}}} \quad (1.14)$$

$$\frac{p_{inj}}{p_i} = 1 + \gamma M_i^2 \quad (1.15)$$

$$\frac{p_t}{(p_{cns})} = (\frac{2}{(\gamma+1)})^{\frac{\gamma}{\gamma-1}} \quad (1.16)$$

$$v_e = \sqrt{\frac{2g\gamma}{\gamma-1}RT_i(1 - \frac{p_e}{p_i})^{\frac{\gamma-1}{\gamma}} + v_i^2} \quad (1.17)$$

$$v_e = \sqrt{\frac{2g\gamma}{\gamma-1}RT_{cns}(1 - \frac{p_e}{(p_{cns})})^{\frac{\gamma-1}{\gamma}}} \quad (1.18)$$

$$Wdot = A_t p_{cns} \sqrt{\frac{g\gamma(\frac{2}{\gamma+1})^{\frac{\gamma}{\gamma-1}}}{RT_{cns}}} \quad (1.19)$$

$$\frac{A_e}{A_t} = \frac{(\frac{2}{\gamma+1})^{\frac{\gamma}{\gamma-1}}(\frac{p_{cns}}{p_e})^{\frac{1}{\gamma}}}{\sqrt{\frac{\gamma+1}{\gamma-1}(1 - (\frac{p_e}{(p_{cns})})^{\frac{\gamma-1}{\gamma}})}} \quad (1.20)$$

$$p_t = (p_{cns})(\frac{2}{\gamma+1})^{\frac{\gamma}{\gamma-1}} \quad (1.21)$$

$$v_t = \sqrt{\frac{2g\gamma}{\gamma+1}RT_{cns}} \quad (1.22)$$

$$\frac{A_x}{A_t} = \frac{1}{M_x} \left(\frac{2}{\gamma+1} \left(1 + \frac{\gamma-1}{2} M_x^2 \right) \right)^{\frac{\gamma+1}{2(\gamma-1)}} \quad (1.24)$$

$$\frac{A_x}{A_t} = \frac{\left(\frac{2}{\gamma+1} \right)^{\frac{1}{\gamma-1}} \left(\frac{(p_{cns})}{p_x} \right)^{\frac{1}{\gamma}}}{\sqrt{\frac{\gamma+1}{\gamma-1} \left(1 - \left(\frac{p_x}{(p_{cns})} \right)^{\frac{\gamma-1}{\gamma}} \right)}} \quad (1.25)$$

$$v_x = \sqrt{\frac{2g\gamma}{\gamma-1}RT_{cns} \left(1 - \left(\frac{p_x}{(p_{cns})} \right)^{\frac{\gamma-1}{\gamma}} \right)} \quad (1.26)$$

$$\frac{v_x}{v_t} = \sqrt{\frac{\gamma+1}{\gamma-1} \left(1 - \frac{p_x}{(p_{cns})} \right)^{\frac{\gamma-1}{\gamma}}} \quad (1.27)$$